---
title: chain homotopy
draft: false
tags:
 - definition
---
# Definition
Given [[202407080950|chain maps]] $f_\bullet, g_\bullet:M_\bullet \to N_\bullet$ between [[202407080919|chain complexes]], a **chain homotopy** is a sequence of group homomorphims 

$$h_n:M_n \longrightarrow N_{n+1}$$

such that 

$$f_n - g_n = d\circ h_n + h_{n-1} \circ d$$

Seen a little clearer in the diagram below
```tikz
\usepackage{tikz-cd}

\tikzcdset{scale cd/.style={every label/.append style={scale=#1},
    cells={nodes={scale=#1}}}}
	
\begin{document}
\begin{tikzcd}[scale cd=2, sep=huge]
\dots \arrow[r, "d"] & M_{n+1} \arrow[r, "d"] 
\arrow[d, "f_{n+1} - g_{n+1}", swap]
& M_n \arrow[r, "d"] \arrow{d}[yshift=6pt]{f_{n} - g_{n}}
\arrow[dl, "h_n"]
& M_{n-1} \arrow[r, "d"] \arrow[dl, "h_{n-1}"]
& \dots\\
\dots \arrow[r, "d"] & N_{n+1} \arrow[r, "d"] 
& N_n \arrow[r, "d"] & N_{n-1} \arrow[r, "d"] & \dots
\end{tikzcd}

\end{document}
```


# Connection to homology
Chain homotopic maps induce the same maps on [[202407080925|homology]].

## Proof
It suffices to prove that
$$
H_i(f_\bullet) = H_i(g_\bullet)
$$
as maps $H_i(M_\bullet) \to H_i(N_\bullet)$. 

Let $[x] \in H_i(M_\bullet)$ with representative $x\in M_i$ (this means that $d_ix = 0$). 

Then 
$$
H_i(f_\bullet)([x]) = [f_i(x)] \quad \text{and} \quad H_i(g_\bullet)([x]) = [g_i(x)]
$$
The homotopy condition gives
$$
\begin{align*}
[f_i(x)] &= [g_i(x) +  d_{i+1} h_i(x) + h_{i-1} d_{i}(x)]\\
&= [g_i(x)]+ [d_{i+1} (h_i(x))] + [0]\\
&= [g_i(x)]
\end{align*}
$$

# Example
Let $R = \mathbb{C}[x,y]$. 
Consider the complex 
$$
0 \longrightarrow R \xrightarrow{\begin{bmatrix}-y \\x\end{bmatrix}} R^{\oplus 2} \xrightarrow{\begin{bmatrix} x & y \end{bmatrix}} R \longrightarrow 0
$$
(note this a $\mathbb{C}[x,y]$-linear [[202501090939|resolution]] of $\mathbb{C}[x,y] \big/ (xy)$ ).

we have a [[202407080950|chain map]] $f_\bullet:M_\bullet \to M_\bullet)$ given by multiplication by $x^2 + y^2$ in each degree. 
$f_\bullet$  is **null-homotopic** (homotopic to the 0 map).

Thus we have the following diagram for the homotopy
```tikz
\usepackage{tikz-cd}
\usepackage{amsmath}
\usepackage{amsfonts}
\let\amsamp=&

\tikzcdset{scale cd/.style={every label/.append style={scale=#1},
    cells={nodes={scale=#1}}}}
	
\begin{document}
\begin{tikzcd}[scale cd=2, sep=huge]
0 \arrow[r] &R\arrow[dl, "0", swap] \arrow[d, "f"] \arrow{r}{\begin{bmatrix}  -y \\x \end{bmatrix}} & R^{\oplus 2} \arrow{dl}[swap]{\begin{bmatrix} -y \amsamp x \end{bmatrix}} \arrow{r}{\begin{bmatrix} x \amsamp y \end{bmatrix}} & R \arrow[r] &0\\
0 \arrow[r] &R \arrow[r] & R^{\oplus 2} \arrow[r] & R \arrow[r] &0

\end{tikzcd}

\end{document}
```
