---
title: equivalent categories
draft: false
tags:
 - definition
---
# Definition
[[202409161019|Categories]] $\mathcal{C}$ and $\mathcal{D}$ are **equivalent** if there exist [[202409162145|functors]] 
$$
F:\mathcal{C} \longrightarrow \mathcal{D}
\quad \text{and} \quad G: \mathcal{D} \longrightarrow \mathcal{C}$$
and [[202409162200|natural isomorphisms]] 
$$
\eta: \text{id}_\mathcal{C} \Longrightarrow G \circ F \quad \text{and} \quad \varepsilon:F \circ G \Longrightarrow \text{id}_\mathcal{D}.
$$

In this case, we call $G$ a **quasi-inverse** of $F$. 

# Conditions for equivalence
A functor $F: \mathcal{C} \to \mathcal{D}$ is part of an equivalence of categories if and only if $F$ is [[202409171519|fully]] [[202406031350|faithful]] and [[202409171525|essentially surjective]].  ^3f61ac

## Proof
#todo

# Examples
## Finite dimensional vector spaces
Let $\text{vect}_k$ be the category of finite dimensional vector spaces over a field $k$ and let $\text{vect}_{k,0}$ be the category of whose objects are the vector spaces $k^n$, $n \geq 0$, and whose morphisms are $k$-linear maps. 
$\text{vect}_k$ and $\text{vect}_{k,0}$ are equivalent.

### Proof
First, we define the functors we will be using. 
We can see that all $\text{obs}(\text{vect}_{k_0}) \subset \text{obs}(\text{vect}_k)$, so the first functor $F$ is the easier one to define. 
$$
\begin{align*}
  F: \text{vect}_{k,0} &\longrightarrow \text{vect}_k \\
  k^n &\longmapsto k^n\\
  k^m \xrightarrow{f} k^n &\longmapsto k^m \xrightarrow{f} k_n
\end{align*}
$$

For the other way, for every $V \in \text{vect}_k$ chose a basis $\{v_i\}$ and let $\varphi_V \in \text{Hom}_{\text{vect}_k}(V, k^{\dim V})$ be the transformation that maps coefficients given the basis $\{v_i\}$  of the standard basis in $k^{\dim V}$. 
Then, we can define the functor
$$
\begin{align*}
  G:  \text{vect}_k &\longrightarrow \text{vect}_{k,0}\\
  V &\longmapsto k^{\dim V}\\
  V \xrightarrow{f} W &\longmapsto k^{\dim V} \xrightarrow{\varphi_W \circ f \circ \varphi_V^{-1}} k^{\dim W}
\end{align*}
$$
Next, to prove equivalence we need to give the natural isomorphisms $\eta: \text{id}_{\text{vect}_{k,0}}\Rightarrow G \circ F$ and $\varepsilon:F \circ G \Rightarrow \text{id}_{\text{vect}_k}$.

For each $x \in \text{vect}_{k,0}$, let $\eta_X:X \to X$ be the identity map on $X$. 
This gives us the following diagram:
```tikz
\usepackage{tikz-cd}
\usepackage{amsmath}

\tikzcdset{scale cd/.style={every label/.append style={scale=#1},
    cells={nodes={scale=#1}}}}
\begin{document}
\begin{tikzcd}[scale cd=2, sep=huge]
  \text{id}_{\text{vect}_{k,0}}(X) \arrow[r, "\text{id}_{\text{vect}_{k,0}}(f)"] &\text{id}_{\text{vect}_{k,0}}(Y) \\
  X \arrow[r, "f"]\arrow[u, phantom, sloped, "="]\arrow[d, "\eta_x = \text{id}_X", swap]& Y\arrow[d, "\eta_Y = \text{id}_Y"]\arrow[u, phantom, sloped, "="]\\
  X \arrow[r, "f"]& Y\\
  G \circ F(X) \arrow[u, phantom, sloped, "="]\arrow[r, "f"]& G \circ F(Y)\arrow[u, phantom, sloped, "="]
\end{tikzcd}
\end{document}
```

In this case it is trivial that the diagram commutes as 
$$\text{id}_Y \circ f = f \circ \text{id}_X$$

Now for the harder one! 
Let $\varepsilon_X = \varphi_X^{-1}$ with $\varphi_X$ defined as above using the chosen basis of $X$.
This gives the following diagram for any $f \in \text{Hom}_{\text{vect}_k}(X, Y)$:
```tikz
\usepackage{tikz-cd}
\usepackage{amsmath}

\tikzcdset{scale cd/.style={every label/.append style={scale=#1},
    cells={nodes={scale=#1}}}}
	
\begin{document}
\begin{tikzcd}[scale cd=2, sep=huge]
F \circ G(X) \arrow[r, "F \circ G(f)"] &F \circ G(Y)\\
k^{\dim X} \arrow[r, "\varphi_Y \circ f \circ \varphi_X^{-1}"]\arrow[u, phantom, sloped, "="]\arrow[d, "\varepsilon_X = \varphi_X^{-1}", swap]& k^{\dim Y}\arrow[d, "\varepsilon_Y = \varphi_Y^{-1}"]\arrow[u, phantom, sloped, "="]\\
X \arrow[r, "f"]& Y\\
\text{id}_{\text{vect}_k}(X) \arrow[u, phantom, sloped, "="]\arrow[r, "\text{id}_{\text{vect}_k}(f)"]& \text{id}_{\text{vect}_k}(Y) \arrow[u, phantom, sloped, "="]
\end{tikzcd}

\end{document}
```

Starting from the upper left hand corner and going right across the top first then down gives
$$\varphi_Y^{-1} \circ \varphi_Y \circ f \circ \varphi_X^{-1} = f \circ \varphi_X^{-1}$$
which is the same as going down first then right along the bottom. 
Therefore, the diagram commutes and $\varepsilon$ is a natural transformation. 

Importantly, $\eta_X$ is an isormophism for each $X \in \text{vect}_{k_0}$ trivially, but $\varepsilon_X = \varphi_X^{-1}$ is also an isomorphism in $\text{vect}_k$ (the inverse is the obvious inverse that must be linear). 
Hence, $\text{vect}_k$ and $\text{vect}_{k,0}$ are equivalent. 
