---
title: trace
draft: false
tags:
 - definition
---
# Coordinate (lame) version
Given a square matrix $A$ the trace is the sum of the diagonal entries, the **trace** of $A$ is 

$$
\text{tr}(A) = \sum_i A_{ii}.
$$

In this form its a bit hard to see why it is important has has some interesting properties. 

# Coordinate free version
For finite dimensional vector spaces $V$ and $W$, there is a canonical isomorphism using the [[20240103134157-tensor_product|tensor product]]

$$
\begin{split}
V^* \otimes W &\longrightarrow \text{Hom}(V, W) \\
\varepsilon \otimes w &\longmapsto \left( \begin{split} f:V &\to W \\
v &\mapsto \varepsilon(v) w \end{split} \right) 
\end{split}
$$

So we can use this idea on the set of linear maps $V \to V$ to make a new linear map $\text{Hom}(V, V) \to \mathbb{C}$. 

$$ 
\begin{split}
\text{Hom}(V, V) \cong V^* \otimes V &\longrightarrow \mathbb{C} \\
f \mapsto \varepsilon \otimes v &\longmapsto \varepsilon(v)
\end{split}
$$

Thus, the **trace** of a linear map $f \in \text{Hom}(V, V)$ is 

$$
tr(f) = \varepsilon(v)
$$

as above. 

## Why is this the trace?
How do these two definitions match?

Given a basis $\{v_1, \dots, v_n\}$ for $V$, then

$$
f(v) = f\left(\sum_i c_i v_i\right) = \sum_i a_i f(v_i)
$$

Then looking at each $f(v_i)$ then we can see that 

$$
f(v_i) = \sum_k^n b_k v_k
$$

So, all together, (combining coefficients) this is equivalent to 

$$
f(v) \cong \sum c_{ij} (v_i^* \otimes v_j)
$$

where $\{v_1^*, \dots, v_n^*\}$ is the [[202403251449|dual basis]]. 

So then, using the definition of the trace, we get 

$$
\begin{align*}
\text{tr}(f) &= \text{tr}\left(\sum c_{ij} (v_i^* \otimes v_j)\right)\\
&= \sum c_{ij} v_i^*(v_j) \\
&= \sum c_{ii}
\end{align*}
$$

since $v_i^*(v_j) = 0$ for $i \neq j$. 
This coincides with the trace formula for a matrix form of a linear map. 

# Properties
1. $\text{tr}: \text{Hom}(V,V)$ is linear 

2. $\text{tr}(\varphi f \varphi^{-1}) = \text{tr}(f)$ for each invertible $\varphi$ 

3. For $f:V \to W$ and $h: W \to V$, $\text{tr}(fh) = \text{tr}(hf)$

4. $\text{tr}(f \oplus g) = \text{tr}(f) + \text{tr}(g)$ 

5. $\text{tr}(f \otimes g) = \text{tr}(f) \cdot \text{tr}(g)$

6. $f: V \to V$ induces $f^*:V^* \to V^*$ and $\text{tr}(f) = \text{tr}(f^*)$

# References
[[@brocker2003]] - Chapter 2 section 3