---
title: tangent space
draft: false
tags:
  - definition
---
# Definition
$$T_pM = \{\varphi \in \mathcal{O}_{M,p}^* \ \big| \ \varphi(\alpha \beta ) = \varphi(\alpha)\beta(p) + \alpha(p)\varphi(\beta) \quad \forall \alpha, \beta \in \mathcal{O}_{M,p}\} $$
Notes: 
- $T_pM$ is the collection of all the [[202403061121|derivations]] 
- $$\varphi \in \mathcal{O}^*_{M,p} \implies \varphi: C^\infty(U \subseteq M) \to \mathbb{R}$$
- In the notation above $\mathcal{O}_M$ denotes the [[202403081144|sheaf]] of smooth functions on M, and $\mathcal{O}_{M,p}$ is the stock where 
$$ \mathcal{O}_{M,p} = \bigg(\bigsqcup_{p\in U \subset M} \mathcal{O}_M(U)\bigg)/\sim$$
Where $(U,f) \sim (V,g)$ if there exists and open neighborhood $W \subset U \cap V$ such that $p \in W$ and $f|_w = g|_w$.
This takes care of compatibility of functions across open sets. 
# Tangent space of $\mathbb{R}^n$
We can show that tangent space at a point $x \in \mathbb{R}^n$ is isomorphic to another copy of $\mathbb{R}^n$. 
## Theorem
Consider the map 
$$\begin{split}
\Phi: \mathbb{R}_a^n &\to T_a\mathbb{R}^n\\
v &\mapsto D_v|_a .
\end{split}
$$
Where $D_v|_a$ is the directional derivative in the direction $v$. 
$\Phi$ is an isomorphism of vector spaces. 
### Proof
**Linearity:** We know that $\Phi$ is linear because 
$$\begin{align*}
\Phi(\vec v + \vec w)(f) &= D_{\vec v+\vec w}|_a(f) \\
& = \nabla f\cdot (\vec v+ \vec w)\\
& = \nabla f \cdot \vec v + \nabla f \cdot \vec w\\
& = \Phi(\vec v)(f) + \Phi(\vec w)(f)
\end{align*}$$
With a similar argument for scalar multiplication. 

**Injective:** Need to show that $\ker \Phi = \{0\}$.
First, note that $\Phi(\vec 0) = \nabla \cdot 0 = 0$. 
Next, let $\vec v \in \ker \Phi$. 
Then 
$$0 = D_v|_a(f) = \nabla f \cdot v \quad \forall f: \mathbb{R^n} \to \mathbb{R}.$$
Let $f$ be the coordinate function that takes the $i$th coordinate to, and all others to 0. 
By the above, $v_i = 0$ for all $i$, so $v = \vec 0$. 

**Surjective:** Let $w \in T_x\mathbb{R}^n$. 
Thus, $w: \mathcal{O}_{\mathbb{R}^n} \to \mathbb{R}$ that is linear and $w(fg) = w(f)g(x) + f(x)w(g)$. 

For any function $f \in \mathcal{O}_{\mathbb{R}^n}$, we can take the Taylor series expansion with 2nd order remainder
$$ \begin{split} f(\vec x) &= f(\vec a) + J(\vec a)(\vec x-\vec a) + R(\vec x) + \\ 
&= f(a) +  \sum_i \frac{\partial f}{\partial x_i}(x_i - a_i) + \sum_{i,j} (x_i - a_i)(x_j - a_j) \int_0^1(1-t)\frac{\partial^2f}{\partial x_i \partial x_j} (a + t(x-a))\end{split}$$

Because $w$ is linear we can look at each term. 
Looking at the last term because $w$ is a derivation, and $f(a)$ is a constant $w\big(f(a)\big) = 0$. 
Also, for the remainder term, 
$$ \begin{align}& w\bigg(\sum_{i,j} (x_i - a_i)(x_j - a_j) \int_0^1(1-t)\frac{\partial^2f}{\partial x_i \partial x_j} (a + t(x-a)) \bigg) \\
&= \sum_{i,j} w\bigg((x_i - a_i)(x_j - a_j) \int_0^1(1-t)\frac{\partial^2f}{\partial x_i \partial x_j} (a + t(x-a)) \bigg)\\
&= \sum_{i,j}w\big((x_i - a_i)\big)(a_j - a_j) \int_0^1(1-t)\frac{\partial^2f}{\partial x_i \partial x_j} (a + t(x-a)) \bigg)\\
& \qquad + \sum(a_i - a_i)w\bigg( (x_j - a_j) \int_0^1(1-t)\frac{\partial^2f}{\partial x_i \partial x_j} (a + t(x-a)) \bigg)\\
&= 0
\end{align}$$
So we only need to look at the middle term. 

Therefore, 
$$\begin{align} w(f) &= w\bigg(\sum_i \frac{\partial f}{\partial x_i}(x_i - a_i))\bigg)\\
&= \sum_i \frac{\partial f}{\partial x_i}\big(w(x_i - a_i)\big)\\
&= \sum_i \frac{\partial f}{\partial x_i}\big(w(x_i) - w(a_i)\big)\\
&= \sum_i \frac{\partial f}{\partial x_i}\big(w(x_i)\big)\\

\end{align}$$
Let $v_i = w(x_i)$ then $\Phi(v) = w$ so $\Phi$ is surjective. 
Hence, it is an isomorphism of vector spaces. 

# Tangent spaces of manifolds
For a [[202403052130|topological manifold]] $M$, the $\dim T_pM = \dim M$. 

# Change in coordinates
Given smooth charts $(U, \varphi)$ and $(V, \psi)$ on $M$, we can change between partial derivatives in the two systems.
Let $(x^1, \dots, x^n)$ be the coordinate functions for $\varphi$, and $(\tilde x^1, \dots, \tilde x^n)$  be coordinate functions for $\psi$.
$$
\begin{align*}
	\frac{\partial}{\partial x^i} &= d(\varphi^{-1})_{\varphi(p)}\left( \frac{\partial}{\partial x^i} \bigg|_{\varphi(p)}\right) \\
	&= d(\psi^{-1})_{\psi(p)} \ \circ \ d(\psi \circ \varphi^{-1})_{\varphi(p)} \left( \frac{\partial}{\partial x^i}\bigg|_{\psi(p)}\right)\\
	&= d(\psi^{-1})_{\psi(p)}\left( \frac{\partial \tilde x^j}{\partial x^i}(\varphi(p)) \frac{\partial}{\partial \tilde x^j}\bigg|_{\psi(p)}\right)\\
	&= \frac{\partial \tilde x^j}{\partial x^i}(\hat p) \frac{\partial}{\partial \tilde x^j}\bigg|_p
\end{align*}
$$

---
### References
[[@lee2013]] provides a good proof of why this works. Though technically he doesn't use the [[202403081144|sheaf]] of smooth functions taking the [[202403081145|stock]] as I learned from Peter. 

