---
title: Cartan's magic formula
draft: false
tags:
---
# Cartan's magic formula
On a [[20231222094707-smooth_manifold|smooth manifold]]$M$, for any smooth [[202404011135|vector field]] $X \in \mathfrak{X}(M)$ and a [[202404061628|differential form]] $\alpha$,
$$ \mathcal{L}_{X}\alpha = d\iota_{X}\alpha + \iota_{X}d\alpha$$
Where $\mathcal{L}_X\alpha$ denotes the [[202405222331|Lie derivative]] of $\alpha$ with respect to $X$, and $\iota_X$ denotes the [[202405222353|interior product]]. 

## Proof
The proof for $k$-differential forms is by induction on $k$.

Consider a 0-form $f\in C^{\infty}(M)$,

$$
d\iota_{X}f + \iota_{X}df = 0 + df(X) = Xf = \mathcal{L}_{X}f.
$$

Next, let $\omega$ be a differential $k$ form.
Assume that Cartan's Magic Formula works for $k-1$ forms.

Given a chart $(U, x^{i})$, we can write $\omega$ locally as

$$
\omega = \sum_{i_{1}\leq \dots \leq i_{k}} \omega_{i_{1}, \dots, i_{k}} d x_{i_{1}} \wedge \dots \wedge dx_{i_{k}}
$$

We want to split this down into smaller forms to use the induction hypothesis, so let $f = x_{i_{1}}$ and $\beta = w_{i_{1}\dots i_{k}} dx_{i_{2}} \wedge \dots \wedge dx_{i_{k}}$

Then we can rewrite each term in the sum above as
$$
\omega_{i_{1}, \dots, i_{k}} d x_{i_{1}} \wedge \dots \wedge x_{i_{k}} =  d x_{i_{1}} \wedge  \omega_{i_{1}, \dots, i_{k}} dx_{i_{2}} \wedge d x_{i_{3}}\dots \wedge d x_{i_{k}} = df \wedge \beta
$$

Now we check the formula for each term in the sum, using the fact that $\iota_{X}$ and $d$ are linear and follow the graded Leibniz rule.
$$
\begin{align*}
d\iota_{X}(df \wedge \beta) + \iota_{X}d(df \wedge \beta)
&= d\big(\iota_{X}df \wedge \beta + (-1)^{1} df \wedge \iota_{X}\beta\big) + \iota_{X}\big(d^{2}f \wedge \beta + (-1)^{1}df \wedge d\beta\big) \\
&= d(Xf \wedge \beta) - d(df \wedge \iota_{X}\beta) - \iota_{X}(df \wedge d\beta)\\
&= dXf \wedge \beta + Xf d\beta - d^{2}f \wedge d\iota_{X}\beta - \\
& \qquad(-1)^{1}df \wedge d\iota_{X}\beta - \iota_{X}df \wedge d\beta - (-1)^{1}df \wedge \iota_{X}d\beta\\
&= dXf \wedge \beta+ Xfd\beta + df \wedge d\iota_{X}\beta - Xfd\beta + df \wedge \iota_{X}d\beta\\
&= dXf \wedge \beta + df \wedge d\iota_{X}\beta + df \wedge \iota_{X}d\beta\\
&= d(Xf) \wedge \beta + df \wedge (d\iota_{X}\beta + \iota_{X}d\beta)\\
&= d(Xf) \wedge \beta + df \wedge \mathcal{L}_{X}\beta\\
&= d(\mathcal{L}_{X}f) \wedge \beta + df \wedge \mathcal{L}_{X}\beta\\
&= \mathcal{L}_{X}df \wedge \beta  + df \wedge \mathcal{L}_{X}\beta\\
&= \mathcal{L}_{X}(df \wedge \beta)
\end{align*}
$$

Therefore, since Cartan's formula holds for each term in the sum, by linearity it holds for the whole $k$ form.