---
title: isomorphism
draft: false
tags:
 - definition
---
# Definition
For a [[202409161019|category]] $\mathcal{C}$, a morphism $f \in \text{Hom}_\mathcal{C}(X,Y)$ is called an **isomorphism** if there exists a morphism $g \in \text{Hom}_\mathcal{C}(Y,X)$ such that 

$$
g \circ f = \text{id}_X \qquad f \circ g = \text{id}_Y.
$$

# Properties of isomorphisms
## Uniqueness of inverse
If $f$ is a morphism, then $g$ given the properties above is unique:

### Proof
Let $f \in \text{Hom}_\mathcal{C}(X,Y)$ be an isomorphism and let $g, \tilde g \in \text{Hom}_\mathcal{C}(Y,X)$ be inverse functions such that
$$
\begin{align*}
g \circ f &= \text{id}_X &\tilde g \circ f = \text{id}_X\\
f \circ g &= \text{id}_Y &f \circ \tilde g = \text{id}_Y\\
\end{align*}
$$

This means that $f \circ g = f \circ \tilde g$. 
Using (associative) composition again with $g$ gives

$$
\begin{align*}
g \circ \left( f \circ g\right) &= g \circ \left( f \circ \tilde g\right)\\
\left( g \circ f \right) \circ g&= \left( g \circ f \right) \circ \tilde g\\
\text{id}_X \circ g &= \text{id}_X \circ \tilde g \\
g &= \tilde g
\end{align*}
$$

Therefore, the inverse function is unique, and we can denote it by $f^{-1}$.

## Inverse of inverse
If $f$ is an isomorphism, then so too is $f^{-1}$ and $(f^{-1})^{-1}=f$.

### Proof
Let $f \in \text{Hom}_\mathcal{C}(X,Y)$ be an isomorphism.
Stated again, this means that $\exists f^{-1}\in \text{Hom}_\mathcal{C}(Y,X)$ such that 
$$ 
  f^{-1} \circ f = \text{id}_X    \quad \text{and} \quad
f \circ f^{-1} = \text{id}_Y$$
To prove $f^{-1}$ is an isomorphism, we need to find a function $g \in \text{Hom}_\mathcal{C}(X,Y)$ such that
$$ 
  g \circ f^{-1} = \text{id}_Y    \quad \text{and} \quad
 f^{-1} \circ g = \text{id}_X$$
 Let $g = f$, thus $(f^{-1})^{-1} = f$.

## Composition of isomorphisms.
If $f \in \text{Hom}_{\mathcal{C}}(X,Y)$ and $g \in \text{Hom}_{\mathcal{C}}(Y,Z)$ are isomorphisms, then so too is $g \circ f \in \text{Hom}_{\mathcal{C}}(X,Z)$.

### Proof
Let  $f \in \text{Hom}_{\mathcal{C}}(X,Y)$ and $g \in \text{Hom}_{\mathcal{C}}(Y,Z)$ be isomorphisms. 
Then there exist morphisms $f^{-1} \in \text{Hom}_{\mathcal{C}}(Y,X)$ and $g^{-1} \in \text{Hom}_{\mathcal{C}}(Z,Y)$
such that 
$$
\begin{align*}
  f \circ f^{-1} &= \text{id}_Y  &g \circ g^{-1} = \text{id}_Z \\
  f^{-1} \circ f &= \text{id}_X  &g^{-1} \circ g = \text{id}_Y
\end{align*}
$$
Then for the morphism $g \circ f$, consider the morphism $f^{-1} \circ g^{-1}$. 
$$
\begin{align*}
  (g \circ f) \circ (f^{-1} \circ g^{-1}) 
  &= g \circ (f \circ f^{-1}) \circ g^{-1} \\
  &= g \circ \text{id}_Y \circ g^{-1}\\
  &= g \circ g^{-1} \\
  &= \text{id}_Z
\end{align*}
$$
and 
$$
\begin{align*}
  (f^{-1} \circ g^{-1}) \circ (g \circ f) 
  &=f^{-1} (\circ g^{-1} \circ g) \circ f \\
  &=f^{-1} \circ \text{id}_Y \circ f \\
  &= \text{id}_X
\end{align*}
$$
Therefore $(f^{-1} \circ g^{-1}) = (g \circ f)^{-1}$ and $g \circ f$ is a morphism. 
