---
title: direct sum
draft: false
tags:
  - definition
status: Cleanup
---
# Overview
Direct sum is a way to make a new algebraic structure (like a [[202403121554|group]], [[202404171457|ring]], [[202409182227|module]], etc.) from existing ones such that the projection should respect the structure of the building blocks. 


# Direct sum of groups
# Direct sum of R-modules
Given two R-modules $M$ and $N$, the direct sum $M \oplus N$ is the set $M \times N$ with the addition defined as the abelian group case. 

The $R$ action is defined by 
$$
r \cdot (m,n) = (r\cdot m, r\cdot n)
$$

## Direct summand
Let $R$ be a ring.
A **direct summand** of an $R$-module $N$ is a submodule $M \subset N$ for which there exists a submodule $P \subset N$ such that $M \oplus P \simeq N$.

### Split inclusion
Let $M$ be a submodule of an $R$-module $N$.
$M$ is a direct summand if and only if the inclusion $i: M \hookrightarrow N$ is **split**, that is, there exists a morphism $s: N \rightarrow M$ which satisfies $s \circ i = \text{id}_M$.

#### Proof
First assume $M$ is a direct summand of $N$, so $N \simeq M \oplus P$. 
Then let $s:M \oplus P \to M$ be the projection in the first element. 
Looking at the maps 
$$
\begin{align*}
M   \hookrightarrow M \oplus P \xrightarrow{ \ s \ } M \\
m \longmapsto (m, 0) \longmapsto m
\end{align*}
$$
$s$ is certainly surjective, and $s \circ i = \text{id}_M$

Next, let there be the morphisms $i, s$ as described in the prompt:
```tikz
\usepackage{tikz-cd}
\usepackage{amsmath}

\tikzcdset{scale cd/.style={every label/.append style={scale=#1},
    cells={nodes={scale=#1}}}}
	
\begin{document}
\begin{tikzcd}[scale cd=2, sep=huge]
M \arrow[rr, bend left = 30, "\text{id}_M"] \arrow[r, "i"]& N \arrow[r, "s"] & M \\
\end{tikzcd}

\end{document}
```

Thus, we know that $i$ must be injective and $s$ must be surjective or else the composition would not be the identity. 

From this we claim that $N \simeq \text{im} \ i \oplus \ker s \simeq M \oplus \ker s$. 
It is clear that $\text{im} \ i \cap \ker s = \{0\}$ since if $n \in \text{im} \ i \cap \ker s$ then $s(n) = 0$ and $i(s(n)) = 0$ where $i$ is injective so $n = 0$. 
Next, let $n \in N$ then we can take $m = s(n)$, using this element, let $n_i = i(m)$. 
Now we can take the element $n_k = n - n_i$. 
$$
s(n_k) = s(n - n_i) = s(n) - s(n_i) = m -m = 0
$$
so $n_k \in \ker s$ and $n = n_i + n_k$. 
Therefore, $N = M \oplus \ker s$. 
